src/ssa/ssa_interpreter.v
@@ -149,8 +149,7 @@ match state with
     | insn_gep id0 inbounds0 t v idxs =>
       do mp <- getOperandValue TD v lc gl;
       do vidxs <- values2GVs TD idxs lc gl;
-      do t' <- getGEPTyp idxs t;
-      do mp' <- GEP TD t mp vidxs inbounds0 t';
+      do mp' <- GEP TD t mp vidxs inbounds0;
          ret ((mkState Sys TD Ps ((mkEC F B cs tmn (updateAddAL _ lc id0 mp') 
                als)::EC) gl fs Mem0), trace_nil)
     | insn_trunc id0 truncop0 t1 v1 t2 =>
@@ -242,8 +241,6 @@ Proof.
     simpl. rewrite H. simpl. rewrite <- H0. simpl. rewrite H1. simpl. auto.
   Case "dsBranch_uncond".
     simpl. rewrite <- H. simpl. rewrite H0. simpl. auto.
-  Case "dsGEP".
-    rewrite H. simpl. rewrite H0. simpl. rewrite H1. simpl. rewrite H2. auto.
   Case "dsCall".
     unfold lookupFdefViaGV in H.
     destruct (getOperandValue TD fv lc gl); try solve [inversion H]. simpl.
@@ -443,9 +440,7 @@ Proof.
           try solve [inversion HinterInsn].         
         remember (values2GVs CurTargetData0 l0 lc Globals0) as R3.
         destruct R3; simpl in HinterInsn; try solve [inversion HinterInsn].     
-        remember (getGEPTyp l0 t) as R4.
-        destruct R4; simpl in HinterInsn; try solve [inversion HinterInsn].
-        remember (GEP CurTargetData0 t g l1 i1 t0) as R2.
+        remember (GEP CurTargetData0 t g l1 i1) as R2.
         destruct R2; simpl in HinterInsn; 
           inversion HinterInsn; subst; eauto.
 
